Added SHL instruction.

src/coq/App/Instruction.v
@@ -10,7 +10,8 @@ Inductive Instruction : Type :=
     | IMM : B64 -> Instruction
     | PUSH : Instruction
     | POP : Instruction
-    | SEL : nat -> Instruction.
+    | SEL : nat -> Instruction
+    | SHL : nat -> Instruction.
 
 (* The time to execute a NOP instruction. *)
 Definition NOP_DELAY : nat := 1.
@@ -26,5 +27,8 @@ Definition POP_DELAY : nat := 2.
 
 (* The time to execute a SEL instruction. *)
 Definition SEL_DELAY : nat := 3.
+
+(* The time to execute a SHL instruction. *)
+Definition SHL_DELAY : nat := 2.
 
 End Instruction.
